testGCD.v
@@ -1,0 +1,95 @@
+From PA Require Import ProgramAlgebra.
+Import Nat.
+Import List.
+Require Import String.
+Import ListNotations.
+
+
+Variable bot : Type.
+
+Record MyVar := mkVar {
+  id: string;
+  val : nat;
+}.
+
+Definition eqVarb (x y : MyVar) := 
+  andb (eqb x.(id) y.(id)) (PeanoNat.Nat.eqb x.(val) y.(val)).
+
+Definition GLOBVARS := [(mkVar "a" 10);(mkVar "b" 4)].
+
+Definition UNDEF := mkVar "Undefined" 0.
+
+Instance myParams : ProgramAlgebra.UserParams :=
+  ProgramAlgebra.Build_UserParams MyVar GLOBVARS eqVarb.
+
+Axiom equalGLOB : GLOBVARS = ProgramAlgebra.GLOBVARS.
+
+Axiom equalB : eqVarb = ProgramAlgebra.eqb.
+
+Notation "|-| l" := (ProgramAlgebra.Choice_of_Alg_List l)(at level 20).
+
+Notation "_|_" := (ProgramAlgebra.Chaos)(at level 10).
+
+Notation "@{ e }" := (fun x => ProgramAlgebra.Assn x e)(at level 10).
+
+Definition gt_a_b : ProgramAlgebra.Boolexp :=
+  fun l =>
+    match (find (fun x => eqb x.(id) "a") l),
+    (find (fun x => eqb x.(id) "b") l) with
+    | Some x, Some y => if (PeanoNat.Nat.leb x.(val) y.(val)) then false else true
+    | _, _ => false
+    end.
+
+Definition gcd_step := ProgramAlgebra.makeAssign ProgramAlgebra.GLOBVARS
+  (fun l =>
+   match (find (fun x => eqb x.(id) "a") l),
+    (find (fun x => eqb x.(id) "b") l) with
+   | Some x, Some y => [(mkVar x.(id) y.(val));(mkVar y.(id) (x.(val) - y.(val)))]
+   | _, _ => []
+   end).
+
+Definition skip := ProgramAlgebra.makeAssign ProgramAlgebra.GLOBVARS
+  (fun l => l).
+
+Fixpoint mapid {s} (x : ProgramAlgebra.Alg s) :=
+  match x with
+  | ProgramAlgebra.Assn _ a => @{a} (ProgramAlgebra.Alg s)
+  | ProgramAlgebra.Choice _ P Q =>
+     ProgramAlgebra.Choice (ProgramAlgebra.Alg s) (mapid P) (mapid Q)
+  | ProgramAlgebra.Chaos _ => _|_ (ProgramAlgebra.Alg s)
+  | ProgramAlgebra.Seq _ P Q =>
+     ProgramAlgebra.Choice (ProgramAlgebra.Alg s) (mapid P) (mapid Q)
+  | ProgramAlgebra.Cond _ P b Q =>
+     ProgramAlgebra.Cond (ProgramAlgebra.Alg s) (mapid P) b (mapid Q)
+  | ProgramAlgebra.Recur _ f => _|_ (ProgramAlgebra.Alg s)
+  end.
+
+Definition testIter {s} (x : ProgramAlgebra.Alg s) :=
+  ProgramAlgebra.Seq (ProgramAlgebra.Alg s)
+  (mapid x) (ProgramAlgebra.Cond (ProgramAlgebra.Alg s)
+     (@{gcd_step} (ProgramAlgebra.Alg s)) gt_a_b
+     (@{skip} (ProgramAlgebra.Alg s))).
+
+Definition testRec := ProgramAlgebra.Recur (ProgramAlgebra.Alg bot) testIter.
+
+Definition testnf := @{ ProgramAlgebra.makeAssign ProgramAlgebra.GLOBVARS 
+  (fun l => [(mkVar "a" 2);(mkVar "b" 2)]) } bot.
+
+Variable lub : ProgramAlgebra.Closure -> ProgramAlgebra.Ualg.
+
+Example testlim : testIter testnf = testRec .
+Proof. unfold testRec. rewrite ProgramAlgebra.Recur_clos with (lub := lub).
+rewrite ProgramAlgebra.fix_is_lub with (lub := lub);auto.
+unfold ProgramAlgebra.RecurFix. unfold testnf. eexists. split.
+unfold testIter. unfold skip. unfold gcd_step.
+rewrite ProgramAlgebra.Assign_Cond. unfold mapid.
+rewrite ProgramAlgebra.Assign_compose. reflexivity.
+unfold gt_a_b. unfold ProgramAlgebra.exp_Cond.
+simpl. unfold ProgramAlgebra.eqEval. auto.
+Qed.
+
+
+
+
+
+
